backend/Unusedglobproof.v
@@ -803,7 +803,11 @@ Lemma external_call_inject:
     /\ Mem.unchanged_on (loc_unmapped f) m1 m2
     /\ Mem.unchanged_on (loc_out_of_reach f m1) m1' m2'
     /\ inject_incr f f'
-    /\ inject_separated f f' m1 m1'.
+    /\ inject_separated f f' m1 m1'
+    /\ (forall b : block,
+          ~ Mem.valid_block m1 b ->
+          Mem.valid_block m2 b ->
+          exists b' : block, f' b = Some (b', 0) /\ Mem.block_compartment m2 b = Some (comp_of ef)).
 Proof.
   intros. eapply external_call_mem_inject_gen; eauto.
   apply globals_symbols_inject; auto.
@@ -1148,7 +1152,7 @@ eapply call_trace_translated; eauto.
   intros (vargs' & P & Q).
   exploit external_call_inject; eauto.
   eapply match_stacks_preserves_globals; eauto.
-  intros (j' & tv & tm' & A & B & C & D & E & F & G).
+  intros (j' & tv & tm' & A & B & C & D & E & F & G & I).
   econstructor; split.
   eapply exec_Ibuiltin; eauto.
   eapply match_states_regular with (j := j'); eauto.
@@ -1203,7 +1207,7 @@ eapply call_trace_translated; eauto.
 - (* external function *)
   exploit external_call_inject; eauto.
   eapply match_stacks_preserves_globals; eauto.
-  intros (j' & tres & tm' & A & B & C & D & E & F & G).
+  intros (j' & tres & tm' & A & B & C & D & E & F & G & I).
   econstructor; split.
   eapply exec_function_external; eauto.
   (* { rewrite <- (match_stacks_call_comp _ _ _ _ _ STACKS); eauto. } *)
