cfrontend/Cminorgenproof.v
@@ -2149,7 +2149,7 @@ Proof.
   exploit match_callstack_match_globalenvs; eauto. intros [hi' MG].
   exploit external_call_mem_inject; eauto.
   eapply inj_preserves_globals; eauto.
-  intros [f' [vres' [tm' [EC [VINJ [MINJ' [UNMAPPED [OUTOFREACH [INCR SEPARATED]]]]]]]]].
+  intros [f' [vres' [tm' [EC [VINJ [MINJ' [UNMAPPED [OUTOFREACH [INCR [SEPARATED COMPNEW]]]]]]]]]].
   left; econstructor; split.
   apply plus_one. econstructor. eauto.
   (* rewrite <- (comp_transl_partial _ TRF). *)
@@ -2316,11 +2316,10 @@ Opaque PTree.set.
   exploit match_callstack_match_globalenvs; eauto. intros [hi MG].
   exploit external_call_mem_inject; eauto.
   eapply inj_preserves_globals; eauto.
-  intros [f' [vres' [tm' [EC [VINJ [MINJ' [UNMAPPED [OUTOFREACH [INCR SEPARATED]]]]]]]]].
+  intros [f' [vres' [tm' [EC [VINJ [MINJ' [UNMAPPED [OUTOFREACH [INCR [SEPARATED COMPNEW]]]]]]]]]].
   left; econstructor; split.
   apply plus_one. econstructor.
-  eapply external_call_symbols_preserved; eauto. apply senv_preserved.
-  econstructor; eauto.
+  eapply external_call_symbols_preserved; eauto. apply senv_preserved. econstructor; eauto.
   apply match_callstack_incr_bound with (Mem.nextblock m) (Mem.nextblock tm).
   eapply match_callstack_external_call; eauto.
   intros. eapply external_call_max_perm; eauto.
