cfrontend/SimplLocalsproof.v
@@ -2271,7 +2271,7 @@ Proof.
 (* builtin *)
   exploit eval_simpl_exprlist; eauto with compat. intros [CASTED [tvargs [C D]]].
   exploit external_call_mem_inject; eauto. apply match_globalenvs_preserves_globals; eauto with compat.
-  intros [j' [tvres [tm' [P [Q [R [S [T [U V]]]]]]]]].
+  intros [j' [tvres [tm' [P [Q [R [S [T [U [V W]]]]]]]]]].
   econstructor; split.
   apply plus_one. econstructor; eauto.
   rewrite <- (comp_transl_partial _ TRF). eauto.
@@ -2461,7 +2461,7 @@ Proof.
   monadInv TRFD. inv FUNTY.
   exploit external_call_mem_inject; eauto. apply match_globalenvs_preserves_globals.
   eapply match_cont_globalenv. eexact (MCONT VSet.empty (comp_of ef)).
-  intros [j' [tvres [tm' [P [Q [R [S [T [U V]]]]]]]]].
+  intros [j' [tvres [tm' [P [Q [R [S [T [U [V W]]]]]]]]]].
   econstructor; split.
   apply plus_one. econstructor; eauto. eapply external_call_symbols_preserved; eauto. apply senv_preserved.
   econstructor; eauto.
